Clean up heap_lang and remove some FIXMEs.
Notable changes:
* I am now using the same names for the fields of the language record and the
  instances in heap_lang. In order to deal with shadowing, I have put all
  definitions in heap_lang.v in a module.
* Instead of defining evaluation contexts recursively, these are now defined
  using lists. This way we can easily reuse operations on lists. For example,
  composition of evaluation contexts is just appending lists. Also, it allowed
  me to simplify the rather complicated proof of step_by_val as induction on
  the shape of contexts no longer results in a blow-up of the number of cases.
* Use better automation to prove all lemmas of heap_lang.
* I have introduced tactics to invert steps and to do steps. These tactics
  greatly helped simplifying boring parts of lifting lemmas.

barrier/sugar.v
@@ -1,5 +1,6 @@
 Require Export barrier.heap_lang barrier.lifting.
 Import uPred.
+Import heap_lang.
 
 (** Define some syntactic sugar. LitTrue and LitFalse are defined in heap_lang.v. *)
 Definition Lam (e : {bind expr}) := Rec e.[ren(+1)].
@@ -13,67 +14,52 @@ Definition Eq e1 e2 :=
 
 Definition LamV (e : {bind expr}) := RecV e.[ren(+1)].
 
-Definition LetCtx (K1 : ectx) (e2 : {bind expr}) := AppRCtx (LamV e2) K1.
-Definition SeqCtx (K1 : ectx) (e2 : expr) := LetCtx K1 (e2.[ren(+1)]).
+Definition LetCtx (e2 : {bind expr}) := AppRCtx (LamV e2).
+Definition SeqCtx (e2 : expr) := LetCtx (e2.[ren(+1)]).
 
 Section suger.
 Context {Σ : iFunctor}.
 Implicit Types P : iProp heap_lang Σ.
-Implicit Types Q : val heap_lang → iProp heap_lang Σ.
+Implicit Types Q : val → iProp heap_lang Σ.
 
 (** Proof rules for the sugar *)
 Lemma wp_lam E ef e v Q :
-  e2v e = Some v → ▷wp E ef.[e/] Q ⊑ wp E (App (Lam ef) e) Q.
+  to_val e = Some v → ▷ wp E ef.[e/] Q ⊑ wp E (App (Lam ef) e) Q.
 Proof.
   intros Hv. rewrite -wp_rec; last eassumption.
   (* RJ: This pulls in functional extensionality. If that bothers us, we have
      to talk to the Autosubst guys. *)
   by asimpl.
 Qed.
-
 Lemma wp_let e1 e2 E Q :
-  wp E e1 (λ v, ▷wp E (e2.[v2e v/]) Q) ⊑ wp E (Let e1 e2) Q.
+  wp E e1 (λ v, ▷wp E (e2.[of_val v/]) Q) ⊑ wp E (Let e1 e2) Q.
 Proof.
-  rewrite -(wp_bind (LetCtx EmptyCtx e2)). apply wp_mono=>v.
-  rewrite -wp_lam //. by rewrite v2v.
+  rewrite -(wp_bind [LetCtx e2]). apply wp_mono=>v.
+  by rewrite -wp_lam //= to_of_val.
 Qed.
-
-Lemma wp_if_true e1 e2 E Q :
-  ▷wp E e1 Q ⊑ wp E (If LitTrue e1 e2) Q.
-Proof.
-  rewrite -wp_case_inl //. by asimpl.
-Qed.
-
-Lemma wp_if_false e1 e2 E Q :
-  ▷wp E e2 Q ⊑ wp E (If LitFalse e1 e2) Q.
-Proof.
-  rewrite -wp_case_inr //. by asimpl.
-Qed.
-
+Lemma wp_if_true e1 e2 E Q : ▷ wp E e1 Q ⊑ wp E (If LitTrue e1 e2) Q.
+Proof. rewrite -wp_case_inl //. by asimpl. Qed.
+Lemma wp_if_false e1 e2 E Q : ▷ wp E e2 Q ⊑ wp E (If LitFalse e1 e2) Q.
+Proof. rewrite -wp_case_inr //. by asimpl. Qed.
 Lemma wp_lt n1 n2 E P Q :
-  (n1 < n2 → P ⊑ ▷Q LitTrueV) →
-  (n1 ≥ n2 → P ⊑ ▷Q LitFalseV) →
+  (n1 < n2 → P ⊑ ▷ Q LitTrueV) →
+  (n1 ≥ n2 → P ⊑ ▷ Q LitFalseV) →
   P ⊑ wp E (Lt (LitNat n1) (LitNat n2)) Q.
 Proof.
-  intros HPlt HPge.
-  rewrite -(wp_bind (LeLCtx EmptyCtx _)) -wp_plus -later_intro. simpl.
-  apply wp_le; intros; [apply HPlt|apply HPge]; omega.
+  intros; rewrite -(wp_bind [LeLCtx _]) -wp_plus -later_intro /=.
+  auto using wp_le with lia.
 Qed.
-
 Lemma wp_eq n1 n2 E P Q :
-  (n1 = n2 → P ⊑ ▷Q LitTrueV) →
-  (n1 ≠ n2 → P ⊑ ▷Q LitFalseV) →
+  (n1 = n2 → P ⊑ ▷ Q LitTrueV) →
+  (n1 ≠ n2 → P ⊑ ▷ Q LitFalseV) →
   P ⊑ wp E (Eq (LitNat n1) (LitNat n2)) Q.
 Proof.
   intros HPeq HPne.
-  rewrite -wp_let -wp_value' // -later_intro. asimpl.
-  rewrite -wp_rec //. asimpl.
-  rewrite -(wp_bind (CaseCtx EmptyCtx _ _)) -later_intro.
-  apply wp_le; intros Hn12.
-  - asimpl. rewrite -wp_case_inl // -!later_intro. apply wp_le; intros Hn12'.
-    + apply HPeq; omega.
-    + apply HPne; omega.
-  - asimpl. rewrite -wp_case_inr // -later_intro -wp_value' //.
-    apply HPne; omega.
+  rewrite -wp_let -wp_value' // -later_intro; asimpl.
+  rewrite -wp_rec //; asimpl.
+  rewrite -(wp_bind [CaseCtx _ _]) -later_intro; asimpl.
+  apply wp_le; intros; asimpl.
+  * rewrite -wp_case_inl // -!later_intro. apply wp_le; auto with lia.
+  * rewrite -wp_case_inr // -later_intro -wp_value' //; auto with lia.
 Qed.
 End suger.
