iris/language.v
@@ -11,7 +11,7 @@ Structure language := Language {
   to_of_val v : to_val (of_val v) = Some v;
   of_to_val e v : to_val e = Some v → of_val v = e;
   values_stuck e σ e' σ' ef : prim_step e σ e' σ' ef → to_val e = None;
-  atomic_not_value e : atomic e → to_val e = None;
+  atomic_not_val e : atomic e → to_val e = None;
   atomic_step e1 σ1 e2 σ2 ef :
     atomic e1 →
     prim_step e1 σ1 e2 σ2 ef →
@@ -24,7 +24,7 @@ Arguments prim_step {_} _ _ _ _ _.
 Arguments to_of_val {_} _.
 Arguments of_to_val {_} _ _ _.
 Arguments values_stuck {_} _ _ _ _ _ _.
-Arguments atomic_not_value {_} _ _.
+Arguments atomic_not_val {_} _ _.
 Arguments atomic_step {_} _ _ _ _ _ _ _.
 
 Canonical Structure istateC Σ := leibnizC (state Σ).
@@ -47,9 +47,7 @@ Section language.
   Lemma reducible_not_val e σ : reducible e σ → to_val e = None.
   Proof. intros (?&?&?&?); eauto using values_stuck. Qed.
   Lemma atomic_of_val v : ¬atomic (of_val v).
-  Proof.
-    by intros Hat; apply atomic_not_value in Hat; rewrite to_of_val in Hat.
-  Qed.
+  Proof. by intros Hat%atomic_not_val; rewrite to_of_val in Hat. Qed.
   Global Instance: Injective (=) (=) (@of_val Λ).
   Proof. by intros v v' Hv; apply (injective Some); rewrite -!to_of_val Hv. Qed.
 End language.
@@ -59,12 +57,12 @@ Instance: Params (@fill) 3.
 Arguments fill {_ _ _} !_ _ / : simpl nomatch.
 
 Class CtxLanguage (Λ : language) (C : Type) `{Fill C (expr Λ)} := {
-  is_ctx_value K e :
+  fill_not_val K e :
     to_val e = None → to_val (fill K e) = None;
-  is_ctx_step_preserved K e1 σ1 e2 σ2 ef :
+  fill_step K e1 σ1 e2 σ2 ef :
     prim_step e1 σ1 e2 σ2 ef →
     prim_step (fill K e1) σ1 (fill K e2) σ2 ef;
-  is_ctx_step K e1' σ1 e2 σ2 ef :
+  fill_step_inv K e1' σ1 e2 σ2 ef :
     to_val e1' = None → prim_step (fill K e1') σ1 e2 σ2 ef →
     ∃ e2', e2 = fill K e2' ∧ prim_step e1' σ1 e2' σ2 ef
 }.
